SystemFD/Examples/Sanity.lean
@@ -13,20 +13,35 @@ def boolCtx : Ctx Term := [
 #eval! wf_ctx boolCtx
 
 def test : Ctx Term := [
-
     .datatype ★
-  -- Just : ∀ a. a → Maybe a
-  ,  .ctor (∀[★] #0 -t> (#3 `@k #1))
-  -- Nothing : ∀ a. Maybe a
-  ,  .ctor (∀[★] #1 `@k #0)
-  -- Maybe : ★ → ★
-  , .datatype  (★ -k> ★)
+  , .ctor (∀[★] #0 -t> (#3 `@k #1))  -- Just : ∀ a. a → Maybe a
+  , .ctor (∀[★] #1 `@k #0)           -- Nothing : ∀ a. Maybe a
+  , .datatype  (★ -k> ★)             -- Maybe : ★ → ★
 
-  , .datatype  (★ -k> ★ -k> ★)
+  , .ctor #1
+  , .ctor #0
+  , .datatype ★
 ]
-#eval! wf_ctx test
+
+#eval wf_ctx test
+
+#eval stable_type_match test (#1 `@t #6) (#1 `@t #6 `@ #5)
 
 #eval infer_type test (((refl! (∀[★]#4 `@k #0))) `@c[refl! #0])
+
+#eval infer_type test (#2 `@t #6)
+#eval infer_type test (#4)
+#eval prefix_type_match test (#3 `@k #6) #6
+#eval infer_type test (.ite (#2 `@t #6) (#2 `@t #6) (#4) (#4))
+
+
+#eval infer_type test (#1 `@t #6 `@ #5)
+#eval infer_type test (#1 `@t #6)
+#eval infer_type test (`λ[#6] #0)
+#eval infer_type test (.ite (#1 `@t #6) (#1 `@t #6 `@ #5) (`λ[#6] #0) (`λ[#6] #0))
+
+
+-- #eval eval_ctx_loop test (.ite (#1 `@t #6) (#1 `@t #6 `@ #5) (`λ[#6] #0) (`λ[#6] #0))
 
 -- #eval eval_ctx_loop test (((refl! (∀[★]#4 `@k #0))) `@c[refl! #0])
 -- #eval eval_ctx_loop test (((refl! (∀[★]∀[★]#6 `@k #1 `@k #0))) `@c[refl! #0] `@c[refl! #0])
